Axiomatic induction-induction gets MSQ further

MichaelScottQ.v
@@ -1,7 +1,198 @@
 Require Import RGref.DSL.DSL.
 Require Import RGref.DSL.Concurrency.
 
-(** A Tail-less Michael-Scott Queue *)
+(** * A Tail-less Michael-Scott Queue *)
+
+(** ** An attempt at axiomatizing an inductive-inductive definition with an induction principle. *)
+Section IndIndAxiomaticHack.
+Axiom Node : Set.
+Axiom validNode : hpred Node.
+Axiom deltaNode : hrel Node.
+Axiom mkNode : nat -> option (ref{Node|validNode}[deltaNode,deltaNode]) -> Node.
+Axiom Node_rect : forall (P:Node->Type), (forall n o, P (mkNode n o)) -> forall nd, P nd. 
+Inductive validNode' : hpred Node :=
+  | nil_next : forall n h, validNode' (mkNode n None) h
+  | nil_reach : forall n h tl, validNode' (h[tl]) h ->
+                               validNode' (mkNode n (Some tl)) h
+with deltaNode' : hrel Node :=
+  | node_nil_refl : forall n h h',
+                  deltaNode' (mkNode n None) (mkNode n None) h h'
+  | node_tl_refl : forall n h h' tl,
+                   deltaNode' (h[tl]) (h'[tl]) h h' ->
+                   deltaNode' (mkNode n (Some tl)) (mkNode n (Some tl)) h h'
+  | node_append : forall n n' tl h h',
+                    (* Do I need this? h[tl]=(mkNode Node validNode R n' None) -> *)
+                    h'[tl]=(mkNode n' None) ->
+                    deltaNode' (mkNode n None)
+                              (mkNode n (Some tl))
+                              h h'.
+Axiom validity : validNode ≡p validNode'.
+Axiom delta_eq : deltaNode ⊆⊇ deltaNode'.
+Inductive msq_reach : forall {T:Set}{P R G} (p:ref{T|P}[R,G]) (a:Node), Prop :=
+  | msq_reach_tail : forall p n, msq_reach p (mkNode n (Some p)).
+(* This instance must be defined this way rather than as a naive match on the node
+   to avoid eliminating a large data type (the inductive-inductive-hacked Node)
+   into Type *)
+Global Instance nd_reach : ImmediateReachability Node := {
+  imm_reachable_from_in := fun T P R G p a => msq_reach p a}.
+
+(** Still need one injectivity axiom to work around the impredicative set stuff... but this axiomatization
+    actually should make the -impredicative-set flag unnecessary.  Might be worth converting the whole framework, though. *)
+Axiom node_inj : forall n n' t t', mkNode n t = mkNode n' t' -> n=n' /\ t=t'.
+Lemma stable_node' : stable validNode' deltaNode'.
+  compute; intros.
+  induction H0; eauto; try constructor.
+      apply IHdeltaNode'. inversion H; subst. assert (Htmp := node_inj _ _ _ _ H2). destruct Htmp. inversion H3.
+                                              assert (Htmp := node_inj _ _ _ _ H1). destruct Htmp. inversion H4; subst. assumption.
+      rewrite H0. constructor.
+Qed.
+Hint Resolve stable_node'.
+
+Definition clean_node_ptr : ref{Node|validNode}[deltaNode,deltaNode] -> ref{Node|validNode'}[deltaNode',deltaNode'].
+  intros.
+  assert (H1 := validity). assert (H2 := delta_eq).
+  compute in *. destruct H2.
+  eapply convert; eauto. intros; firstorder.
+Defined.
+Definition noderef := ref{Node|validNode}[deltaNode,deltaNode].
+  
+(** We're following The Art of Multiprocessor Programming, S10.5, but
+    temporarily skipping the tail.
+    Enqueue appends a single node at the end.
+    Dequeue moves the head pointer froma sentinel to sentinel.next, which
+    becomes the new sentinel.
+*)
+Inductive MSQ : Set := mkMSQ : noderef -> MSQ.
+Definition vMSQ : hpred MSQ := any. (* More interesting with tail pointer *)
+Inductive δmsq : hrel MSQ :=
+  (* h and h' here are important.  This allows arbitrary changes as long as the
+     head pointer remains unchanged.  It relies on the noderef to enforce
+     further properties. *)
+  | msq_nop : forall n h h', δmsq n n h h'
+  | msq_dequeue : forall n hd h h' rest,
+                    h[hd]=(mkNode n (Some rest)) ->
+                    δmsq (mkMSQ hd) (mkMSQ rest) h h'.
+Definition msq := ref{MSQ|vMSQ}[δmsq,δmsq].
+Inductive q_reachability : forall {T:Set}{P R G} (p:ref{T|P}[R,G]) (q:MSQ), Prop :=
+  | q_r : forall n, q_reachability n (mkMSQ n).
+Instance q_reach : ImmediateReachability MSQ :=
+  { imm_reachable_from_in := @q_reachability }.
+
+Lemma MSQ_stability : stable vMSQ δmsq.
+Proof.
+  compute; intros; eauto.
+Qed.
+Hint Resolve MSQ_stability.
+Check @contains.
+Inductive nd_contains : hrel Node -> Prop :=
+  | nd_cont : forall RR n tl,
+                @contains noderef _ (fun c c' h h' => RR (mkNode n (Some tl))
+                                              (mkNode n (Some tl))
+                                              h h') ->
+              nd_contains RR.
+Instance nd_containment : Containment Node := { contains := nd_contains }.
+Inductive msq_contains : hrel MSQ -> Prop :=
+  | msq_cont : forall RR tl,
+                contains (fun c c' h h' => RR (mkMSQ tl) (mkMSQ tl) h h') ->
+              msq_contains RR.
+Instance msq_containment : Containment MSQ := { contains := msq_contains }.
+Instance nd_fold : rel_fold Node.
+  (* TODO: Again, need a workaround for the ind-ind hack + constructor typing args. *)
+Print rel_fold.
+  eapply Build_rel_fold. intros. exact H.
+Defined.
+Instance msq_fold : rel_fold MSQ.
+  (* TODO: Again, need a workaround for the ind-ind hack + constructor typing args. *)
+  eapply Build_rel_fold. intros. exact H.
+Defined.
+
+Lemma precise_valid_node : precise_pred validNode'.
+  compute. intros; intuition; eauto. induction H; constructor.
+  rewrite <- H0; try solve[repeat constructor]. 
+  eapply IHvalidNode'. intros.
+  Require Import Coq.Program.Equality.
+  dependent induction H1.
+    (* This case is a messy contradiction, induction tried to use the reflexively reachable case for things w/ wrong types *) admit.
+    eapply H0. eapply trans_reachable with (i := tl). constructor. eapply directly_reachable. assumption.
+    eapply H0. clear IHreachable_from_in. eapply trans_reachable with (i := tl). constructor. eapply trans_reachable with (i := i); eauto.
+Qed.
+Hint Resolve precise_valid_node.
+
+Lemma precise_delta_node : precise_rel deltaNode'.
+  compute; intros; intuition; eauto. induction H1; try constructor.
+
+  rewrite <- H. rewrite <- H0. apply IHdeltaNode'.
+  intros. apply H. eapply trans_reachable with (i := tl). constructor. assumption.
+  intros. apply H0. eapply trans_reachable with (i := tl). constructor. assumption.
+  constructor. constructor. constructor. constructor.
+
+  eapply node_append.
+  rewrite <- H0. eauto.
+  constructor. constructor.
+Qed.
+Hint Resolve precise_delta_node.
+Lemma precise_valid_node2 : precise_pred validNode.
+Proof. compute. assert (Htmp := validity). compute in Htmp.
+       assert (forall x h, validNode x h -> validNode' x h). intros; edestruct Htmp; eauto.
+       assert (forall x h, validNode' x h -> validNode x h). intros; edestruct Htmp; eauto.
+       intros.
+       apply H0. eapply precise_valid_node; eauto.
+Qed.
+Lemma precise_delta_node2 : precise_rel deltaNode.
+Proof. compute. assert (Htmp := delta_eq). destruct Htmp. compute in *.
+       intros. apply H0. eapply precise_delta_node; eauto.
+Qed.
+Hint Resolve precise_valid_node2 precise_delta_node2.
+Lemma delta_refl : hreflexive deltaNode.
+Proof. compute. intros. destruct delta_eq. apply H0.
+       (* TODO: This may actually be false at the moment; need to fix this *)
+Admitted.
+Hint Resolve delta_refl.
+
+Lemma precise_δmsq : precise_rel δmsq.
+  compute; intros. induction H1; eauto; try constructor.
+  eapply msq_dequeue. rewrite <- H. apply H1. constructor. constructor.
+Qed.
+Lemma precise_vMSQ : precise_pred vMSQ.
+  compute; intros. auto.
+Qed.
+Hint Resolve precise_δmsq precise_vMSQ.
+Local Obligation Tactic := intros; intuition; eauto; try repeat constructor.
+
+Lemma stability : stable validNode deltaNode.
+Proof. red. intros. destruct (validity x' h'). destruct delta_eq; compute in *.
+       apply H2.
+       eapply stable_node'; eauto.
+       destruct (validity x h). firstorder.
+Qed.
+Hint Resolve stability.
+
+Program Definition alloc_msq {Γ} (_:unit) : rgref Γ msq Γ :=
+  sentinel <- Alloc (mkNode 0 None);
+  Alloc (mkMSQ sentinel).
+Next Obligation. destruct (validity (mkNode 0 None) h). apply H1; constructor. Qed.
+
+Program Definition dq_msq {Γ} (q:msq) : rgref Γ (option nat) Γ :=
+  RGFix _ _ (fun rec q =>
+    match !q with
+    | mkMSQ sent =>
+      Node_rect (fun _ => _) (fun x o => match o return (!sent=mkNode x o) -> rgref Γ (option nat) Γ with
+                                         | None => fun _ => rgret None
+                                         | Some hd => fun _ =>
+                                               Node_rect (fun _ => _) (fun n tl => success <- CAS(q,mkMSQ sent,mkMSQ hd);
+                                                                                   if success then rgret (Some n) else rec q) (!hd)
+                                         end eq_refl) (!sent)
+    end) q.
+Next Obligation. (* δmsq guarantee proof *)
+  apply msq_dequeue with (n := x). (* TODO: Follows from appropriate !x=h[x] assumption... *) admit.
+Qed.
+Next Obligation. subst. (* TODO: Need to fix up induction principle for this to work right. *) admit.
+Qed.
+(* TODO: PROBLEM: folding the δmsq restriction through the list when finding the tail to enqueue means δmsq must account for enqueues.
+   Currently it doesn't. *)
+
+
+End IndIndAxiomaticHack.
 
 (** Unless we introduce lots of indirections through references to options,
     we're stuck adapting Capretta's impredicative induction-recursion
